

## TD 1: Exercises on multivariate statistics and regression

## ► Exercise 1

Let  $U$  and  $V$  be two independent random variables with uniform distribution over  $[0, 1]$ .

Let  $X = U + V$  and  $Y = U - V$ .

- (a) Compute the expectation and covariance matrix of  $Z = \begin{pmatrix} X & Y \end{pmatrix}^T$ .

$$Z = \begin{bmatrix} X \\ Y \end{bmatrix} \Rightarrow \mathbb{E}[Z] = \begin{bmatrix} \mathbb{E}[X] \\ \mathbb{E}[Y] \end{bmatrix} = \begin{bmatrix} \mathbb{E}[U + V] \\ \mathbb{E}[U - V] \end{bmatrix} = \begin{bmatrix} \mathbb{E}[U] + \mathbb{E}[V] \\ \mathbb{E}[U] - \mathbb{E}[V] \end{bmatrix}$$

Remember that

$$\mathbb{E}[U] = \int_{\mathbb{R}} u p_U(u) du = \int_0^1 u du = \frac{1}{2} = \mathbb{E}[V] \quad \text{therefore} \quad \mathbb{E}[Z] = \begin{bmatrix} 1 \\ 0 \end{bmatrix}$$

We also have that

$$\text{cov}(Z) = \Sigma_Z = \mathbb{E}[(Z - \mathbb{E}[Z])(Z - \mathbb{E}[Z])^T] = \begin{bmatrix} \text{Var}(X) & \text{Cov}(X, Y) \\ \text{Cov}(X, Y) & \text{Var}(Y) \end{bmatrix}$$

Since  $U$  and  $V$  are independent, we can write

$$\begin{aligned} \text{Var}(X) &= \text{Var}(U + V) = \text{Var}(U) + \text{Var}(V) \\ \text{Var}(Y) &= \text{Var}(U - V) = \text{Var}(U) + \text{Var}(V) \end{aligned}$$

and remember the definition of variance

$$\text{Var}(U) = \int_{\mathbb{R}} (u - \mathbb{E}[u])^2 p_U(u) du = \frac{1}{12} = \text{Var}(V)$$

Now we have to calculate the cross-covariance,

$$\text{Cov}(X, Y) = \mathbb{E}_{XY}[(X - \mathbb{E}[X])(Y - \mathbb{E}[Y])] = \mathbb{E}[(X - 1)Y] = \mathbb{E}[XY] - \mathbb{E}[Y] = \mathbb{E}[U^2 - V^2]$$

and finally

$$\text{Cov}(X, Y) = \mathbb{E}[U^2] - \mathbb{E}[V^2] = 0 \quad \text{therefore} \quad \Sigma_Z = \begin{bmatrix} \frac{1}{6} & 0 \\ 0 & \frac{1}{6} \end{bmatrix}$$

- (b) Prove that  $X$  and  $Y$  are uncorrelated but not independent.

From the result in (a) we see that  $\text{Cov}(X, Y) = 0$  so they are indeed uncorrelated.

To check whether two random variables are independent we have to first calculate their joint pdf  $p_{XY}(x, y)$  and compare it to the marginal pdfs  $p_X(x)$  and  $p_Y(y)$ . The random variables will be independent **\*\*if, and only if,\*\*** we can write  $p_{XY}(x, y) = p_X(x)p_Y(y)$

First, recall that

$$\begin{aligned} X &= U + V \\ Y &= U - V \end{aligned} \iff \begin{aligned} U &= \frac{1}{2}(X + Y) \\ Y &= \frac{1}{2}(X - Y) \end{aligned}$$

So let's first check what is the joint pdf. We can simply use the transformation method, which writes

$$p_{XY}(x, y) = p_{UV}(u, v) \times |\det(J)|^{-1}$$

where  $J$  is the jacobian of the transformation from  $(U, V)$  to  $(X, Y)$ :

$$J = \begin{bmatrix} \frac{\partial X}{\partial U} & \frac{\partial X}{\partial V} \\ \frac{\partial Y}{\partial U} & \frac{\partial Y}{\partial V} \end{bmatrix} = \begin{bmatrix} 1 & 1 \\ 1 & -1 \end{bmatrix} \Rightarrow |\det(J)| = 2$$

Then

$$p_{XY}(x, y) = p_U\left(\frac{1}{2}(x+y)\right)p_V\left(\frac{1}{2}(x-y)\right) \times \frac{1}{2}$$

We thus identify a pdf which is constant on a region  $\mathcal{S}$  defined by the two uniform marginals. Let's see what  $\mathcal{S}$  looks like:

Since  $0 \leq U \leq 1$  and  $0 \leq V \leq 1$ , then we have  $0 \leq X+Y \leq 2$  and  $0 \leq X-Y \leq 2$ , therefore  $0 \leq X \leq 2$  and  $-X \leq Y \leq X$

So we can write the joint pdf as per

$$p_{XY}(x, y) = \begin{cases} \frac{1}{2}, & 0 \leq x \leq 2 \quad -x \leq y \leq x \\ 0, & \text{otherwise} \end{cases}$$

OK, we have the joint pdf. Let's see now what the marginal for  $X$  looks like.

Remember that  $X = U + V$  with  $U$  and  $V$  independent. One way of calculating the pdf for the sum of two general RVs is to begin with the CDF and then taking its derivative. Let's see where this gets us:

$$F_X(x) = \mathbb{P}(X \leq x) = \mathbb{P}(U + V \leq x) = \iint_{u+v \leq x} p_{UV}(u, v) du dv = \int_{-\infty}^{+\infty} \int_{-\infty}^{x-u} p_U(u) p_V(v) du dv$$

Rearranging things, we get

$$F_X(x) = \int_{-\infty}^{+\infty} p_U(u) \left( \int_{-\infty}^{x-u} p_V(v) dv \right) du = \int_{-\infty}^{+\infty} p_U(u) F_V(x-u) du$$

So the pdf of  $X$  can be calculated as

$$p_X(x) = \frac{d}{dx} F_X(x) = \int_{-\infty}^{+\infty} p_U(x) \left( \frac{d}{dx} F_V(x-u) \right) du = \int_{-\infty}^{+\infty} p_U(x) p_V(x-u) du$$

For our specific case with two uniform distributions, this gives

$$p_X(x) = \int_0^1 p_V(x-u) du = \int_0^1 \mathbf{1}_{[0,1]}(x-u) du = \begin{cases} 0 & x \leq 0 \quad \text{or} \quad x \geq 2 \\ x & 0 \leq x \leq 1 \\ 2-x & 1 \leq x \leq 2 \end{cases}$$

We see right away that  $p_X(x)$  is not a constant, so we don't even need to calculate the marginal for  $Y$  to conclude that we can not factorize the joint pdf into the marginals. Conclusion, the two RVs are not independent.

## ► Exercise 2

Let  $Z = \begin{pmatrix} X & Y \end{pmatrix}^T$  be a Gaussian vector with mean  $\mu = \begin{pmatrix} 1 & 2 \end{pmatrix}^T$  and covariance  $\Sigma = \begin{pmatrix} 1 & -1 \\ -1 & 2 \end{pmatrix}$ .

- (a) Compute the probability density function of  $Z$ .

The pdf of a bivariate normal distribution is

$$p_Z(\mathbf{z}) = \frac{1}{2\pi \det(\Sigma)} \exp\left(-\frac{1}{2}(\mathbf{z} - \mu)^\top \Sigma^{-1}(\mathbf{z} - \mu)\right)$$

With  $\det(\Sigma) = 1$  and  $\Sigma^{-1} = \begin{bmatrix} 2 & 1 \\ 1 & 1 \end{bmatrix}$

We end up with

$$p_Z(x, y) = \frac{1}{2\pi} \exp\left(-\frac{1}{2}(2x^2 + y^2 + 2xy - 8x - 6y + 10)\right)$$

- (b) Using

$$f_{Y|X=x}(y) = \frac{f_{(X,Y)}(x, y)}{f_X(x)}$$

compute the distribution of  $Y$  given  $X = x$ .

The conditional expectation can be written as

$$p_{Y|X=x}(y) = \frac{p_{XY}(x, y)}{p_X(x)} \quad \text{with} \quad p_X(x) = \frac{1}{\sqrt{2\pi}} \exp\left(-\frac{1}{2}(x-1)^2\right)$$

Which after lots of simplifications gives us:

$$p_{Y|X=x}(y) = \frac{1}{\sqrt{2\pi}} \exp\left(-\frac{1}{2}\left(y - (3-x)\right)^2\right) = \mathcal{N}(y \mid 3-x, 1)$$

- (c) What is the best prediction of  $Y$  given  $X = x$ ?

Remember from the CM1 that the best prediction of  $Y$  given  $X = x$  is the conditional expectation as per

$$\hat{Y} = \mathbb{E}[Y \mid X = x] = 3 - x$$

### ► Exercise 3

Consider the regression problem discussed in class: we want to determine a function  $\mu$  that takes a predictor  $X$  as input and gives the best estimate in terms of mean squared error for the observed variable  $Y$ .

In mathematical terms, we have an optimization problem defined as

$$\mu = \operatorname{argmin}_{f \in \mathcal{F}} \mathbb{E}_{(X,Y)} \left[ \left( Y - f(X) \right)^2 \right]$$

where  $\mathcal{F}$  is a space of functions with finite squared norm.

Show that the solution is  $\mu(x) = \mathbb{E}_{Y|X}[Y \mid X = x]$

We can rewrite the loss function to minimize as per

$$\begin{aligned} \mathbb{E}_{(X,Y)} \left[ (Y - f(X))^2 \right] &= \mathbb{E}_X \left[ \mathbb{E}_{Y|X} \left[ (Y - f(X))^2 \mid X \right] \right] \\ &= \mathbb{E}_X \left[ \operatorname{Var}(Y - f(X) \mid X) + \left( \mathbb{E}_{Y|X} [Y - f(X) \mid X] \right)^2 \right] \\ &= \mathbb{E}_X \left[ \operatorname{Var}(Y \mid X) + \left( \mathbb{E}_{Y|X} [Y - f(X) \mid X] \right)^2 \right] \\ &\geq \mathbb{E}_X \left[ \operatorname{Var}(Y \mid X) \right] \end{aligned}$$

so we see that to minimize the loss we should choose  $f(x) = \mathbb{E}_{Y|X}[Y \mid X = x]$

## ► Exercise 4

Consider the Gaussian simple linear regression model presented in class

$$Y = \beta_0 + \beta_1 X_1 + \varepsilon \quad \text{with} \quad \varepsilon \sim \mathcal{N}(0, \sigma^2)$$

The estimates for the parameters of the model,  $\hat{\beta}_0$  and  $\hat{\beta}_1$ , are obtained  $N$  paired samples  $(x_i, y_i)$ .

(a) Show that the estimated parameters are unbiased.

From the CM we have the expressions

$$\hat{\beta}_0 = \bar{Y} - \hat{\beta}_1 \bar{X} \quad \text{and} \quad \hat{\beta}_1 = \frac{c_{XY}}{s_X^2} \quad \text{with} \quad c_{XY} = \frac{1}{N} \sum_{i=1}^N (x_i - \bar{x})(y_i - \bar{y}) \quad \text{and} \quad s_X^2 = \frac{1}{N} \sum_{i=1}^N (x_i - \bar{x})^2$$

We first check the unbiasedness of  $\hat{\beta}_1$

$\mathbb{E}[\hat{\beta}_1] = \mathbb{E}_{X_1, \dots, X_N} [\mathbb{E}[\hat{\beta}_1 \mid X_1 = x_1, \dots, X_N = x_N]]$  (explain why we first consider the conditional expectation)

$$\mathbb{E}[\hat{\beta}_1 \mid X_1 = x_1, \dots, X_N = x_N] = \frac{1}{s_X^2} \frac{1}{N} \sum_{i=1}^N (x_i - \bar{x}) \left( \mathbb{E}[Y_i \mid X_i = x_i] - \mathbb{E}[\bar{y} \mid X_1 = x_1, \dots, X_N = x_N] \right)$$

(the  $X$  are fixed but the  $Y$  are random variables)

Note that,

$$\mathbb{E}[Y_i \mid X_i = x_i] = \beta_0 + \beta_1 x_i + \mathbb{E}[\varepsilon_i] = \beta_0 + \beta_1 x_i$$

and that

$$\mathbb{E}[\bar{y} \mid X_1 = x_1, \dots, X_N = x_N] = \mathbb{E} \left[ \frac{1}{N} \sum_{i=1}^N (\beta_0 + \beta_1 x_i + \varepsilon_i) \right] = \beta_0 + \beta_1 \bar{x}$$

so we get

$$\mathbb{E}[\hat{\beta}_1 \mid X_1 = x_1, \dots, X_N = x_N] = \frac{1}{s_X^2} \frac{1}{N} \sum_{i=1}^N (x_i - \bar{x}) (\beta_0 + \beta_1 x_i - \beta_0 - \beta_1 \bar{x}) = \beta_1$$

Then taking the expectation along all possible datasets, we get

$$\mathbb{E}[\hat{\beta}_1] = \mathbb{E}_{X_1, \dots, X_N} [\beta_1] = \beta_1$$

The bias for  $\hat{\beta}_0$  is checked similarly.

$$\mathbb{E}[\hat{\beta}_0 \mid X_1 = x_1, \dots, X_N = x_N] = \mathbb{E}[\bar{Y} - \hat{\beta}_1 \bar{X} \mid X_1 = x_1, \dots, X_N = x_N]$$

Which then gives us

$$\mathbb{E}[\bar{Y} \mid X_1 = x_1, \dots, X_N = x_N] = \beta_0 + \beta_1 \bar{x}$$

and

$$\mathbb{E}[\hat{\beta}_1 \bar{X} \mid X_1 = x_1, \dots, X_N = x_N] = \bar{x} \mathbb{E}[\hat{\beta}_1 \mid X_1 = x_1, \dots, X_N = x_N] = \beta_1 \bar{x}$$

so in the end we get

$$\mathbb{E}[\hat{\beta}_0 \mid X_1 = x_1, \dots, X_N = x_N] = \beta_0 + \beta_1 \bar{x} - \beta_1 \bar{x} = \beta_0$$

(b) Show that

$$\text{Var}(\hat{\beta}_1) = \frac{\sigma^2}{N} \frac{1}{s_X^2} \quad \text{and} \quad \text{Var}(\hat{\beta}_0) = \frac{\sigma^2}{N} \left( 1 + \frac{\bar{X}^2}{s_X^2} \right)$$

where  $\bar{X} = \frac{1}{N} \sum_{i=1}^N x_i$  and  $s_X^2 = \frac{1}{N} \sum_{i=1}^N (x_i - \bar{X})^2$ .

OK, now let's get the variances.

Remember that  $\hat{\beta}_1 = \frac{c_{XY}}{s_X^2} = \left( \frac{1}{N} \sum_i x_i y_i - \bar{x} \bar{y} \right) \frac{1}{s_X^2}$  so we will first rewrite it so that things get easier later

Note that

$$y_i = \beta_0 + \beta_1 x_i + \varepsilon_i \quad \text{and} \quad \bar{y} = \beta_0 + \beta_1 \bar{x} + \bar{\varepsilon} \quad \text{where} \quad \bar{\varepsilon} = \frac{1}{N} \sum_i \varepsilon_i$$

and that

$$\frac{1}{N} \sum_i x_i y_i = \frac{1}{N} \sum_i x_i (\beta_0 + \beta_1 x_i + \varepsilon_i) = \beta_0 \bar{x} + \beta_1 \frac{1}{N} \sum_i x_i^2 + \frac{1}{N} \sum_i x_i \varepsilon_i$$

and

$$\bar{x} \bar{y} = \beta_0 \bar{x} + \beta_1 (\bar{x})^2 + \bar{x} \bar{\varepsilon}$$

Then

$$\hat{\beta}_1 = \left( \beta_1 s_X^2 + \frac{1}{N} \sum_i x_i \varepsilon_i - \bar{x} \bar{\varepsilon} \right) \frac{1}{s_X^2} = \beta_1 + \frac{1}{s_X^2} \frac{1}{N} \sum_i (x_i - \bar{x}) \varepsilon_i$$

This way of rewriting the estimator  $\hat{\beta}_1$  is very insightful, since now we can easily write that

$$\text{Var}(\hat{\beta}_1) = \mathbb{E}_{X_1, \dots, X_N} \left[ \text{Var}_X(\hat{\beta}_1 \mid X_1 = x_1, \dots, X_N = x_N) \right] = \mathbb{E}_{X_1, \dots, X_N} \left[ \frac{1}{s_X^4} \frac{1}{N^2} \sum_i (x_i - \bar{x})^2 \sigma^2 \right]$$

so we get

$$\text{Var}(\hat{\beta}_1) = \frac{1}{N^2} \frac{1}{s_X^4} s_X^2 N s_X^2 \sigma^2 = \frac{1}{N} \frac{\sigma^2}{s_X^2}$$

What about  $\hat{\beta}_0$  ?

$$\hat{\beta}_0 = \bar{y} - \hat{\beta}_1 \bar{x} = \left( \beta_0 + \beta_1 \bar{x} + \bar{\varepsilon} \right) - \left( \beta_1 + \frac{1}{s_X^2} \frac{1}{N} \sum_i (x_i - \bar{x}) \varepsilon_i \right) \bar{x}$$

which gives us

$$\hat{\beta}_0 = \beta_0 + \bar{\varepsilon} - \frac{1}{s_X^2} \frac{1}{N} \sum_i (x_i - \bar{x}) \bar{x} \varepsilon_i$$

Therefore,

$$\text{Var}(\hat{\beta}_0) = \frac{\sigma^2}{N} + \frac{1}{N^2 s_X^4} \sum_i (x_i - \bar{x})^2 \bar{x}^2 \sigma^2 = \frac{1}{N} \sigma^2 \left( 1 + \frac{\bar{x}^2}{s_X^2} \right)$$

Using the estimated parameters, we can predict that for a given arbitrary value of  $X$ , say  $x$  (sometimes called the operation point), we have that on average  $Y$  will be

$$\hat{m}(x) = \hat{\beta}_0 + \hat{\beta}_1 x$$

(c) Show that

$$\mathbb{E}[\hat{m}(x)] = \beta_0 + \beta_1 x$$

$$\hat{m}(x) = \hat{\beta}_0 + \hat{\beta}_1 x = (\bar{y} - \hat{\beta}_1 \bar{x}) + \hat{\beta}_1 x = \bar{y} + \hat{\beta}_1 (x - \bar{x})$$

Taking back the expression from item (b)

$$\begin{aligned}
\hat{m}(x) &= \bar{y} + \left( \beta_1 + \frac{1}{s_X^2} \frac{1}{N} \sum_i (x_i - \bar{x}) \varepsilon_i \right) (x - \bar{x}) \\
&= \frac{1}{N} \sum_i \left( \beta_0 + \beta_1 x_i + \varepsilon_i \right) + \left( \beta_1 + \frac{1}{s_X^2} \frac{1}{N} \sum_i (x_i - \bar{x}) \varepsilon_i \right) (x - \bar{x}) \\
&= \beta_0 + \beta_1 \bar{x} + \bar{\varepsilon} + \beta_1 x - \beta_1 \bar{x} + \frac{(x - \bar{x})}{N s_X^2} \sum_i (x_i - \bar{x}) \varepsilon_i \\
&= \beta_0 + \beta_1 x + \bar{\varepsilon} + \frac{(x - \bar{x})}{N s_X^2} \sum_i (x_i - \bar{x}) \varepsilon_i \\
\mathbb{E}[\hat{m}(x)] &= \beta_0 + \beta_1 x
\end{aligned}$$

- (d) Show that the variance of  $\hat{m}(x)$  conditioned on a given choice of datapoints  $x_1, \dots, x_N$  can be written as per

$$\text{Var}_X(\hat{m}(x)) = \frac{\sigma^2}{N} \left( 1 + \frac{(x - \bar{x})^2}{s_X^2} \right)$$

Describe how the variance changes for different choices of the operation point.

Finally, the conditional variance on a given choice of dataset  $x_1, \dots, x_N$  is

$$\text{Var}_X(\hat{m}(x)) = \text{Var}_X \left( \beta_0 + \beta_1 x + \bar{\varepsilon} + \frac{(x - \bar{x})}{N s_X^2} \sum_i (x_i - \bar{x}) \varepsilon_i \right)$$

which can be simplified as per

$$\begin{aligned}
\text{Var}_X(\hat{m}(x)) &= \text{Var} \left( \frac{1}{N} \sum_i \varepsilon_i + \frac{(x - \bar{x})}{N s_X^2} \sum_i (x_i - \bar{x}) \varepsilon_i \right) \\
&= \text{Var} \left( \frac{1}{N} \sum_i \left[ 1 + \frac{(x - \bar{x})}{s_X^2} (x_i - \bar{x}) \right] \varepsilon_i \right) \\
&= \text{Var} \left( \frac{1}{N} \sum_i \left[ 1 + \frac{(x - \bar{x})}{s_X^2} (x_i - \bar{x}) \right] \varepsilon_i \right) \\
&= \frac{1}{N^2} \sum_i \left[ 1 + \frac{(x - \bar{x})}{s_X^2} (x_i - \bar{x}) \right]^2 \text{Var}(\varepsilon_i) \\
&= \frac{\sigma^2}{N^2} \sum_i \left( 1 + \frac{2(x - \bar{x})(x_i - \bar{x})}{s_X^2} + \frac{(x - \bar{x})^2 (x_i - \bar{x})^2}{s_X^4} \right) \\
&= \frac{\sigma^2}{N} \sum_i \left( 1 + \frac{(x - \bar{x})^2}{s_X^2} \right)
\end{aligned}$$

Notice that to get the unconditional variance we would have to take the expectation with respect to the  $x_i$ , which can be quite cumbersome and not that much insightful. We won't do that.